petrinet.v
@@ -1,0 +1,80 @@
+From iris.base_logic Require Export invariants.
+From iris.algebra Require Import auth frac agree gmap.
+From iris_io Require Export lang rules.
+From iris.proofmode Require Import tactics.
+
+Section PetriNet.
+
+  Context `{EqDecision Pl}.
+
+  Inductive Transition : Type :=
+    IOTr (p : Pl) (t : ioTag) (v v' : val) (q : Pl)
+  | SplitTr (p q q': Pl)
+  | JoinTr (p p' q: Pl)
+  | NoOpTr (p q : Pl).
+
+  Definition PetriNet := Transition → Prop.
+
+  Definition Valuation := Pl → nat.
+
+  Implicit Types N : PetriNet.
+  Implicit Types V : Valuation.
+  Implicit Types p q : Pl.
+
+  Definition singVAL p := (λ q, if decide (p = q) then 1 else 0).
+
+  Definition ValPlus V V' := λ p, V p + V' p.
+
+  Notation "V ⊎ W" := (ValPlus V W) (at level 50, left associativity).
+
+  Inductive Traces N : Valuation → ioSpec :=
+  | EmpTR V : Traces N V []
+  | IOTR V p t v v' q τ :
+      N (IOTr p t v v' q) →
+      Traces N ((singVAL q) ⊎ V) τ →
+      Traces N ((singVAL p) ⊎ V) ((t, v, v') :: τ)
+  | SplitTR V p q q' τ :
+      N (SplitTr p q q') →
+      Traces N (singVAL q ⊎ singVAL q' ⊎ V) τ →
+      Traces N (singVAL p ⊎ V) τ
+  | JoinTR V p p' q τ :
+      N (JoinTr p p' q) →
+      Traces N (singVAL q ⊎ V) τ →
+      Traces N (singVAL p ⊎ singVAL p' ⊎ V) τ
+  | NoOpTR V p q τ :
+      N (NoOpTr p q) →
+      Traces N (singVAL q ⊎ V) τ →
+      Traces N (singVAL p ⊎ V) τ.
+
+  Definition ResultDet N V :=
+    ∀ t v v' v'' τ,
+      Traces N V (τ ++ [(t, v, v')]) →
+      Traces N V (τ ++ [(t, v, v'')]) → v' = v''.
+
+  (** The CMRA for petrinet valuations. *)
+  Class petrinetIG Σ := PetriNetIG {
+    PNI_exclG :> inG Σ (authUR (ofe_funUR (λ p : Pl, natUR)));
+    γPN : gname
+  }.
+
+  Context `{petrinetIG Σ}.
+
+  Program Definition FullVAL V :=
+    @own Σ (authUR (ofe_funUR (λ p, natUR))) _ γPN (● V).
+
+  Definition ownVAL V :=
+    @own Σ (authUR (ofe_funUR (λ p, natUR))) _ γPN (◯ V).
+
+  Definition Token p := ownVAL (singVAL p).
+
+  Lemma OwnVAL_split V V' : ownVAL (V ⊎ V') ⊣⊢ ownVAL V ∗  ownVAL V'.
+  Proof. by rewrite /ownVAL -own_op -auth_frag_op. Qed.
+
+  Context {N}.
+
+  
+
+End PetriNet.
+
+Notation "V ⊎ W" := (ValPlus V W) (at level 50, left associativity).
+
